Partially reworked lookup functions and theorems

post-cip/formal-crypto/lean/src/Leioscrypto/FaitAccompli.lean
@@ -1,52 +1,17 @@
 
 import Leioscrypto.BLS
 import Leioscrypto.LocalSortition
+import Leioscrypto.Registration
+import Leioscrypto.StakeDistribution
 import Leioscrypto.Types
 
 
 namespace Leioscrypto
 
 
-structure StakeDistribution where
-  pools : List (PoolKeyHash × Coin)
-  not_duplicated : (pools.map Prod.fst).Nodup
-  have_stake : ∀ stake ∈ pools.map Prod.snd, stake > 0
-  sorted_nonincreasing : pools.Pairwise $ fun ⟨ poolId₁ , stake₁ ⟩ ⟨ poolId₂ , stake₂ ⟩ ↦ stake₁ > stake₂ ∨ stake₁ = stake₂ ∧ poolId₁ > poolId₂
-
-namespace StakeDistribution
-
-  def valid_id (stakes : StakeDistribution) (poolId : PoolKeyHash) : Prop := poolId ∈ stakes.pools.map Prod.fst
-
-  def valid_index (stakes : StakeDistribution) (i : PoolIndex) : Prop := i < stakes.pools.length
-
-  def lookup (stakes : StakeDistribution) (i : PoolIndex) (h : i < stakes.pools.length) : PoolKeyHash × Coin :=
-    stakes.pools.get ⟨ i, h ⟩
-
-  def lookupPoolId (stakes : StakeDistribution) (i : PoolIndex) (h : i < stakes.pools.length) : PoolKeyHash :=
-    Prod.fst $ stakes.pools.get ⟨ i , h ⟩
-
-  def lookupStake (stakes : StakeDistribution) (poolId : PoolKeyHash) : Coin :=
-    (stakes.pools.find? (fun x ↦ x.fst == poolId)).elim 0 Prod.snd
-
-  theorem poolId_in_pools (stakes : StakeDistribution) (i : PoolIndex) (h : i < stakes.pools.length) : lookupPoolId stakes i h ∈ stakes.pools.map Prod.fst :=
-    by
-      let poolId := stakes.lookupPoolId i h
-      rw [lookupPoolId]
-      apply List.mem_map_of_mem
-      apply List.get_mem
-
-  def total (stakes : StakeDistribution): Coin :=
-    (stakes.pools.map Prod.snd).sum
-
-  def remaining (stakes : StakeDistribution) : List Coin :=
-    Prod.fst
-      $ stakes.pools.foldr (init := ([], 0))
-        fun ⟨ _ , stake ⟩ (acc, previousTotal) =>
-          let newTotal := stake + previousTotal
-          (newTotal :: acc, newTotal)
-
-end StakeDistribution
-
+structure WeightedPublicKey where
+  publicKey : BLS.PublicKey
+  weight : Rat
 
 def PoolWeights := List (PoolKeyHash × Rat)
 deriving Inhabited
@@ -129,6 +94,12 @@ namespace FaitAccompli
         let seats := countSeats fa.n₂ 𝒮 σ_eid
         guard $ seats > 0
         pure $ fa.nonpersistentStake * seats
+
+  def weighPersistent (fa : FaitAccompli) (poolIndex : PoolIndex) (h : fa.valid_persistent_id poolIndex) : WeightedPublicKey :=
+    sorry
+
+  def weighNonpersistent (fa : FaitAccompli) (poolId : PoolKeyHash) : WeightedPublicKey :=
+    sorry
 
 end FaitAccompli
 
