post-cip/formal-crypto/lean/src/Leioscrypto/Certificate.lean
@@ -26,14 +26,15 @@ namespace Certificate
     correct_ebhash : c.ebHash = election.ebHash
     unique_persistent_voters : c.persistentVotes.Nodup
     unique_nonpersistent_voters : (c.nonpersistentVotes.map Prod.fst).Nodup
-    valid_persistent_ids : ∀ poolIndex ∈ c.persistentVotes, election.epoch.stakes.valid_index poolIndex
+    valid_persistent_ids : ∀ poolIndex ∈ c.persistentVotes, election.epoch.valid_index poolIndex
     valid_persistent_voters : ∀ poolIndex ∈ c.persistentVotes, election.epoch.fa.valid_persistent_id poolIndex
     valid_nonpersistent_candidates : ∀ poolId ∈ c.nonpersistentVotes.map Prod.fst, election.epoch.fa.valid_nonpersistent_pool poolId
 
-  /-
   def Authentic (c : Certificate) (election : Election) : Prop :=
     let epoch := election.epoch
     let fa := epoch.fa
+
+/-
     let σ_m : BLS.Signature := BLS.AKey c.persistentVotes
     let weighPersistent (poolIndex : PoolIndex) : Option Rat :=
       do
@@ -44,9 +45,9 @@ namespace Certificate
     | ⟨ poolId , σ_eid ⟩ => fa.voteWeight poolId (some σ_eid)
     let nonpersistentWeight : Option Rat :=
       List.sum <$> c.nonpersistentVotes.mapM weighNonpersistent
+-/
     let has_quorum := sorry
     has_quorum
-  -/
 
 end Certificate
 
