post-cip/formal-crypto/lean/src/Leioscrypto/StakeDistribution.lean
@@ -1,0 +1,47 @@
+
+import Leioscrypto.Registration
+import Leioscrypto.Types
+
+
+namespace Leioscrypto
+
+
+structure StakeDistribution where
+  pools : List (PoolKeyHash × Coin)
+  not_duplicated : (pools.map Prod.fst).Nodup
+  have_stake : ∀ stake ∈ pools.map Prod.snd, stake > 0
+  sorted_nonincreasing : pools.Pairwise $ fun ⟨ poolId₁ , stake₁ ⟩ ⟨ poolId₂ , stake₂ ⟩ ↦ stake₁ > stake₂ ∨ stake₁ = stake₂ ∧ poolId₁ > poolId₂
+
+namespace StakeDistribution
+
+  def valid_poolid (stakes : StakeDistribution) (poolId : PoolKeyHash) : Prop := poolId ∈ stakes.pools.map Prod.fst
+
+  def valid_poolindex (stakes : StakeDistribution) (poolIndex : PoolIndex) : Prop := poolIndex < stakes.pools.length
+
+  def lookupPoolId (stakes : StakeDistribution) (poolIndex : PoolIndex) (h : poolIndex < stakes.pools.length) : PoolKeyHash :=
+    Prod.fst $ stakes.pools.get ⟨ poolIndex , h ⟩
+
+  def lookupStake (stakes : StakeDistribution) (poolId : PoolKeyHash) (h : stakes.valid_poolid poolId) : Coin :=
+    lookup₁ stakes.pools poolId h
+
+  theorem poolindex_in_pools (stakes : StakeDistribution) (poolId : PoolIndex) (h : stakes.valid_poolindex poolId) : lookupPoolId stakes poolId h ∈ stakes.pools.map Prod.fst :=
+    by
+      let poolId := stakes.lookupPoolId poolId h
+      rw [lookupPoolId]
+      apply List.mem_map_of_mem
+      apply List.get_mem
+
+  def total (stakes : StakeDistribution): Coin :=
+    (stakes.pools.map Prod.snd).sum
+
+  def remaining (stakes : StakeDistribution) : List Coin :=
+    Prod.fst
+      $ stakes.pools.foldr (init := ([], 0))
+        fun ⟨ _ , stake ⟩ (acc, previousTotal) =>
+          let newTotal := stake + previousTotal
+          (newTotal :: acc, newTotal)
+
+end StakeDistribution
+
+
+end Leioscrypto
